



$$\begin{array}{lll}
 A = (0, 0) & G = (\frac{1}{\sqrt{2}} - \frac{1}{2}, \frac{1}{2}) & M = (1 - \frac{1}{\sqrt{2}} + \frac{1}{2}, \frac{1}{2}) \\
 B = (0, 1) & H = (0, \frac{1}{\sqrt{2}}) & N = (1, 1 - \frac{1}{\sqrt{2}}) \\
 C = (1, 1) & I = (1 - \frac{1}{\sqrt{2}}, 1) & O = (\frac{1}{\sqrt{2}}, 0) \\
 D = (1, 0) & J = (\frac{1}{2}, 1 - \frac{1}{\sqrt{2}} + \frac{1}{2}) & P = (\frac{1}{2}, \frac{1}{\sqrt{2}} - \frac{1}{2}) \\
 E = (1 - \frac{1}{\sqrt{2}}, 0) & K = (\frac{1}{\sqrt{2}}, 1) & \\
 F = (0, 1 - \frac{1}{\sqrt{2}}) & L = (1, \frac{1}{\sqrt{2}}) &
 \end{array}$$